wip: super erasure

lang_ghost.v
@@ -31,20 +31,20 @@ Fixpoint ghost_ok(e: expr): Prop :=
     var_erases_to (true :: gs) (S x) x'
   .
 
-  Inductive erases_to: list bool -> expr -> Plang.expr -> Prop :=
+  Inductive erases_to: list bool -> expr -> expr -> Prop :=
   | Var_erases_to gs x x':
     var_erases_to gs x x' ->
-    erases_to gs (Var x) (Plang.Var x')
+    erases_to gs (Var x) (Var x')
   | Rec_erases_to gs e e':
     erases_to (false :: false :: gs) e e' ->
-    erases_to gs (Rec e) (Plang.Rec e')
+    erases_to gs (Rec e) (Rec e')
   | Lam_erases_to gs e e':
     erases_to (false :: gs) e e' ->
-    erases_to gs (Lam e) (Plang.Lam e')
+    erases_to gs (Lam e) (Lam e')
   | LetIn_erases_to gs e1 e2 e1' e2':
     erases_to gs e1 e1' ->
     erases_to (false :: gs) e2 e2' ->
-    erases_to gs (LetIn e1 e2) (Plang.LetIn e1' e2')
+    erases_to gs (LetIn e1 e2) (LetIn e1' e2')
   | GRLetIn_erases_to gs e1 e2 e2':
     ghost_ok e1 ->
     erases_to (true :: gs) e2 e2' ->
@@ -52,7 +52,7 @@ Fixpoint ghost_ok(e: expr): Prop :=
   | Seq_erases_to gs e1 e2 e1' e2':
     erases_to gs e1 e1' ->
     erases_to gs e2 e2' ->
-    erases_to gs (Seq e1 e2) (Plang.Seq e1' e2')
+    erases_to gs (Seq e1 e2) (Seq e1' e2')
   | GRSeq_erases_to gs e1 e2 e2':
     ghost_ok e1 ->
     erases_to gs e2 e2' ->
@@ -60,81 +60,191 @@ Fixpoint ghost_ok(e: expr): Prop :=
   | App_erases_to gs e1 e2 e1' e2':
     erases_to gs e1 e1' ->
     erases_to gs e2 e2' ->
-    erases_to gs (App e1 e2) (Plang.App e1' e2')
+    erases_to gs (App e1 e2) (App e1' e2')
   | Unit_erases_to gs:
-    erases_to gs Unit Plang.Unit
+    erases_to gs Unit Unit
   | Nat_erases_to gs n:
-    erases_to gs (Nat n) (Plang.Nat n)
+    erases_to gs (Nat n) (Nat n)
   | Bool_erases_to gs b:
-    erases_to gs (Bool b) (Plang.Bool b)
+    erases_to gs (Bool b) (Bool b)
   | BinOp_erases_to gs op e1 e2 e1' e2':
     erases_to gs e1 e1' ->
     erases_to gs e2 e2' ->
-    erases_to gs (BinOp op e1 e2) (Plang.BinOp op e1' e2')
+    erases_to gs (BinOp op e1 e2) (BinOp op e1' e2')
   | If_erases_to gs e0 e1 e2 e0' e1' e2':
     erases_to gs e0 e0' ->
     erases_to gs e1 e1' ->
     erases_to gs e2 e2' ->
-    erases_to gs (If e0 e1 e2) (Plang.If e0' e1' e2')
+    erases_to gs (If e0 e1 e2) (If e0' e1' e2')
   | Pair_erases_to gs e1 e2 e1' e2':
     erases_to gs e1 e1' ->
     erases_to gs e2 e2' ->
-    erases_to gs (Pair e1 e2) (Plang.Pair e1' e2')
+    erases_to gs (Pair e1 e2) (Pair e1' e2')
   | Fst_erases_to gs e e':
     erases_to gs e e' ->
-    erases_to gs (Fst e) (Plang.Fst e')
+    erases_to gs (Fst e) (Fst e')
   | Snd_erases_to gs e e':
     erases_to gs e e' ->
-    erases_to gs (Snd e) (Plang.Snd e')
+    erases_to gs (Snd e) (Snd e')
   | InjL_erases_to gs e e':
     erases_to gs e e' ->
-    erases_to gs (InjL e) (Plang.InjL e')
+    erases_to gs (InjL e) (InjL e')
   | InjR_erases_to gs e e':
     erases_to gs e e' ->
-    erases_to gs (InjR e) (Plang.InjR e')
+    erases_to gs (InjR e) (InjR e')
   | Case_erases_to gs e0 e1 e2 e0' e1' e2':
     erases_to gs e0 e0' ->
     erases_to (false :: gs) e1 e1' ->
     erases_to (false :: gs) e2 e2' ->
-    erases_to gs (Case e0 e1 e2) (Plang.Case e0' e1' e2')
+    erases_to gs (Case e0 e1 e2) (Case e0' e1' e2')
   | Fold_erases_to gs e e':
     erases_to gs e e' ->
-    erases_to gs (Fold e) (Plang.Fold e')
+    erases_to gs (Fold e) (Fold e')
   | Unfold_erases_to gs e e':
     erases_to gs e e' ->
-    erases_to gs (Unfold e) (Plang.Unfold e')
+    erases_to gs (Unfold e) (Unfold e')
   | TLam_erases_to gs e e':
     erases_to gs e e' ->
-    erases_to gs (TLam e) (Plang.TLam e')
+    erases_to gs (TLam e) (TLam e')
   | TApp_erases_to gs e e':
     erases_to gs e e' ->
-    erases_to gs (TApp e) (Plang.TApp e')
+    erases_to gs (TApp e) (TApp e')
   | Fork_erases_to gs e e':
     erases_to gs e e' ->
-    erases_to gs (Fork e) (Plang.Fork e')
+    erases_to gs (Fork e) (Fork e')
   | Loc_erases_to gs l:
-    erases_to gs (Loc l) (Plang.Loc l)
+    erases_to gs (Loc l) (Loc l)
   | IOtag_erases_to gs t:
-    erases_to gs (IOtag t) (Plang.IOtag t)
+    erases_to gs (IOtag t) (IOtag t)
   | Alloc_erases_to gs e e':
     erases_to gs e e' ->
-    erases_to gs (Alloc e) (Plang.Alloc e')
+    erases_to gs (Alloc e) (Alloc e')
   | Load_erases_to gs e e':
     erases_to gs e e' ->
-    erases_to gs (Load e) (Plang.Load e')
+    erases_to gs (Load e) (Load e')
   | Store_erases_to gs e1 e2 e1' e2':
     erases_to gs e1 e1' ->
     erases_to gs e2 e2' ->
-    erases_to gs (Store e1 e2) (Plang.Store e1' e2')
+    erases_to gs (Store e1 e2) (Store e1' e2')
   | CAS_erases_to gs e0 e1 e2 e0' e1' e2':
     erases_to gs e0 e0' ->
     erases_to gs e1 e1' ->
     erases_to gs e2 e2' ->
-    erases_to gs (CAS e0 e1 e2) (Plang.CAS e0' e1' e2')
+    erases_to gs (CAS e0 e1 e2) (CAS e0' e1' e2')
   | Rand_erases_to gs:
-    erases_to gs Rand Plang.Rand
+    erases_to gs Rand Rand
   | IO_erases_to gs e1 e2 e1' e2':
     erases_to gs e1 e1' ->
     erases_to gs e2 e2' ->
-    erases_to gs (IO e1 e2) (Plang.IO e1' e2')
+    erases_to gs (IO e1 e2) (IO e1' e2')
   .
+
+  Inductive val_erases_to: val -> val -> Prop :=
+  | RecV_erases_to e e':
+    erases_to (false :: false :: []) e e' ->
+    val_erases_to (RecV e) (RecV e')
+  | LamV_erases_to e e':
+    erases_to (false :: []) e e' ->
+    val_erases_to (LamV e) (LamV e')
+  | UnitV_erases_to:
+    val_erases_to UnitV UnitV
+  | NatV_erases_to n:
+    val_erases_to (NatV n) (NatV n)
+  | BoolV_erases_to b:
+    val_erases_to (BoolV b) (BoolV b)
+  | PairV_erases_to v1 v2 v1' v2':
+    val_erases_to v1 v1' ->
+    val_erases_to v2 v2' ->
+    val_erases_to (PairV v1 v2) (PairV v1' v2')
+  | InjLV_erases_to v v':
+    val_erases_to v v' ->
+    val_erases_to (InjLV v) (InjLV v')
+  | InjRV_erases_to v v':
+    val_erases_to v v' ->
+    val_erases_to (InjRV v) (InjRV v')
+  | FoldV_erases_to v v':
+    val_erases_to v v' ->
+    val_erases_to (FoldV v) (FoldV v')
+  | TLamV_erases_to e e':
+    erases_to [] e e' ->
+    val_erases_to (TLamV e) (TLamV e')
+  | LocV_erases_to l:
+    val_erases_to (LocV l) (LocV l)
+  | IOtagV_erases_to t:
+    val_erases_to (IOtagV t) (IOtagV t).
+
+  Inductive ectx_item_erases_to: ectx_item -> ectx_item -> Prop :=
+  | AppLCtx_erases_to e e' :
+      erases_to [] e e' →
+      ectx_item_erases_to (AppLCtx e) (AppLCtx e')
+  | AppRCtx_erases_to v v' :
+      val_erases_to v v' →
+      ectx_item_erases_to (AppRCtx v) (AppRCtx v')
+  | LetInCtx_erases_to e e' :
+      erases_to [] e e' →
+      ectx_item_erases_to (LetInCtx e) (LetInCtx e')
+  | SeqCtx_erases_to e e' :
+      erases_to [] e e' →
+      ectx_item_erases_to (SeqCtx e) (SeqCtx e')
+  | TAppCtx_erases_to :
+      ectx_item_erases_to TAppCtx TAppCtx
+  | PairLCtx_erases_to e e' :
+      erases_to [] e e' →
+      ectx_item_erases_to (PairLCtx e) (PairLCtx e')
+  | PairRCtx_erases_to v v' :
+      val_erases_to v v' →
+      ectx_item_erases_to (PairRCtx v) (PairRCtx v')
+  | BinOpLCtx_erases_to op e e' :
+      erases_to [] e e' →
+      ectx_item_erases_to (BinOpLCtx op e) (BinOpLCtx op e')
+  | BinOpRCtx_erases_to op v v' :
+      val_erases_to v v' →
+      ectx_item_erases_to (BinOpRCtx op v) (BinOpRCtx op v')
+  | FstCtx_erases_to :
+      ectx_item_erases_to FstCtx FstCtx
+  | SndCtx_erases_to :
+      ectx_item_erases_to SndCtx SndCtx
+  | InjLCtx_erases_to :
+      ectx_item_erases_to InjLCtx InjLCtx
+  | InjRCtx_erases_to :
+      ectx_item_erases_to InjRCtx InjRCtx
+  | CaseCtx_erases_to e1 e1' e2 e2' :
+      erases_to (false :: []) e1 e1' →
+      erases_to (false :: []) e2 e2' →
+      ectx_item_erases_to (CaseCtx e1 e2) (CaseCtx e1' e2')
+  | IfCtx_erases_to e1 e1' e2 e2' :
+      erases_to [] e1 e1' →
+      erases_to [] e2 e2' →
+      ectx_item_erases_to (IfCtx e1 e2) (IfCtx e1' e2')
+  | FoldCtx_erases_to :
+      ectx_item_erases_to FoldCtx FoldCtx
+  | UnfoldCtx_erases_to :
+      ectx_item_erases_to UnfoldCtx UnfoldCtx
+  | AllocCtx_erases_to :
+      ectx_item_erases_to AllocCtx AllocCtx
+  | LoadCtx_erases_to :
+      ectx_item_erases_to LoadCtx LoadCtx
+  | StoreLCtx_erases_to e e' :
+      erases_to [] e e' →
+      ectx_item_erases_to (StoreLCtx e) (StoreLCtx e')
+  | StoreRCtx_erases_to v v' :
+      val_erases_to v v' →
+      ectx_item_erases_to (StoreRCtx v) (StoreRCtx v')
+  | CasLCtx_erases_to e2 e2' e3 e3' :
+      erases_to [] e2 e2' →
+      erases_to [] e3 e3' →
+      ectx_item_erases_to (CasLCtx e2 e3) (CasLCtx e2' e3')
+  | CasMCtx_erases_to v1 v1' e3 e3' :
+      val_erases_to v1 v1' →
+      erases_to [] e3 e3' →
+      ectx_item_erases_to (CasMCtx v1 e3) (CasMCtx v1' e3')
+  | CasRCtx_erases_to v1 v1' v2 v2' :
+      val_erases_to v1 v1' →
+      val_erases_to v2 v2' →
+      ectx_item_erases_to (CasRCtx v1 v2) (CasRCtx v1' v2')
+  | IOLCtx_erases_to e e' :
+      erases_to [] e e' →
+      ectx_item_erases_to (IOLCtx e) (IOLCtx e')
+  | IORCtx_erases_to v v' :
+      val_erases_to v v' →
+      ectx_item_erases_to (IORCtx v) (IORCtx v').
